add iprop automation and spanning tree predicates

IrisCore/Invariant.thy
@@ -7,7 +7,7 @@ subsection \<open> Invariants \<close>
 
 text \<open>The modular invariant camera based on the heap camera\<close>
 definition own_inv :: "inv \<Rightarrow> iprop" ("Own\<^sub>i _") where
-  "own_inv i = Own(\<epsilon>,\<epsilon>,i,\<epsilon>)"
+  "own_inv i = Own(constr_inv i)"
 
 context assumes "SORT_CONSTRAINT('c::ucamera)" and "SORT_CONSTRAINT('v::ofe)"
 begin
@@ -17,7 +17,7 @@ definition ownI :: "name \<Rightarrow> iprop \<Rightarrow> iprop" where
   "ownI \<iota> P = Own\<^sub>i (fragm [\<iota>\<mapsto>to_ag (Next (pre P))],\<epsilon>,\<epsilon>)"
 
 definition inv :: "namespace \<Rightarrow> iprop \<Rightarrow>  iprop" where
-  "inv N P = \<exists>\<^sub>u \<iota>. ((\<upharpoonleft>(\<iota>\<in>names N)) \<and>\<^sub>u ownI \<iota> P)"
+  "inv N P \<equiv> \<exists>\<^sub>u \<iota>. ((\<upharpoonleft>(\<iota>\<in>names N)) \<and>\<^sub>u ownI \<iota> P)"
   
 text \<open>Allocate new enabled invariant map\<close>
 definition ownE :: "name dset \<Rightarrow> iprop" where
@@ -40,13 +40,42 @@ end
 
 lemma persistent_ownI: "persistent (ownI \<iota> P)"
   unfolding ownI_def own_inv_def by (rule persistent_core_own2)
-  (auto simp add: prod_pcore_id_pred \<epsilon>_pcore_id_def fragm_core_id simp del: \<epsilon>_dfset_def \<epsilon>_dset_def)
+  (auto simp add: prod_pcore_id_pred \<epsilon>_pcore_id_def fragm_core_id constr_inv_def 
+      simp del: \<epsilon>_dfset_def \<epsilon>_dset_def \<epsilon>_option_def)
 
-lemma "persistent (inv N P)"
+lemma persistent_inv: "persistent (inv N P)"
   unfolding inv_def
   apply (rule persistent_exists)
   apply (rule allI)
   apply (rule persistent_conj)
   apply (rule persistent_pure)
   by (rule persistent_ownI)
+
+
+subsubsection \<open>Cancelable Invariants\<close>
+type_synonym cinvG = frac
+definition cinv_own :: "frac \<Rightarrow> iprop" where "cinv_own p = Own (constr_cinv (Some p))"
+definition cinv :: "namespace \<Rightarrow> iprop \<Rightarrow> iprop" where "cinv N P = inv N (P \<or>\<^sub>u cinv_own 1)"
+
+lemma cinv_persistent: "persistent (cinv N P)"
+  unfolding cinv_def by (rule persistent_inv)
+
+lemma timeless_cinv_own: "timeless (cinv_own p)"
+unfolding timeless_def cinv_own_def constr_cinv_def except_zero_def
+apply transfer
+by (simp add: n_incl_incl del: \<epsilon>_dfset_def \<epsilon>_dset_def)
+
+lemma cinv_own_valid: "upred_holds (cinv_own q1 -\<^emph> cinv_own q2 -\<^emph> \<upharpoonleft>(q1\<cdot>q2\<le>1))"
+unfolding cinv_own_def
+apply (rule upred_entails_wand_holdsR2[OF _ own_valid2])
+apply (simp add: constr_cinv_def op_prod_def \<epsilon>_left_id op_option_def del: \<epsilon>_dfset_def \<epsilon>_dset_def)
+apply (simp add: upred_entails.rep_eq upred_valid.rep_eq upred_pure.rep_eq prod_n_valid_def \<epsilon>_n_valid del: \<epsilon>_dfset_def \<epsilon>_dset_def)
+apply (simp add: valid_raw_option_def valid_frac[symmetric] split: option.splits)
+by (metis dcamera_valid_iff less_eq_frac.rep_eq one_frac.rep_eq one_frac_def valid_raw_frac.rep_eq)
+
+lemma cinv_own_1_l: "upred_holds (cinv_own 1 -\<^emph> cinv_own q -\<^emph> \<upharpoonleft>False)"
+proof (rule upred_wand_holds2I)
+  from one_op have "(1\<cdot>q \<le> 1) \<longleftrightarrow> False" by (simp add: less_le_not_le)
+  with upred_wand_holds2E[OF cinv_own_valid, of 1 q] show "cinv_own 1 \<^emph> cinv_own q \<turnstile> \<upharpoonleft>False" by simp
+qed
 end
