IrisCore/iPropShallow.thy
@@ -15,16 +15,145 @@ begin
 *)
 
 type_synonym 'a pre_inv = "(name\<rightharpoonup>'a later ag) auth \<times> name dset \<times> name dfset"
-type_synonym ('a,'b) resF = "graphUR auth \<times> markingUR auth \<times> 'a pre_inv \<times> heap_lang_heap"
 
-text \<open> Axiomatic fixed point definition of iprop.\<close>
-typedecl pre_iprop
-instance pre_iprop :: ofe sorry
-type_synonym inv = "pre_iprop pre_inv"
-type_synonym res = "(pre_iprop,pre_iprop) resF"
-type_synonym iprop = "res upred_f"
+ML \<open>
+  local
+  type camera_data = {
+    camera: typ,
+    name: string,
+    getter: term option,
+    constructor: term option
+  }
 
-axiomatization iProp :: "pre_iprop \<Rightarrow> iprop" and pre :: "iprop \<Rightarrow> pre_iprop"
+  type cameras_data = {
+    number: int,
+    cameras: camera_data list,
+    cmraPT: typ option
+  }
+
+    (* Names *)
+  val iPropN = Binding.name "iProp"
+  val preN = Binding.name "pre"
+  val pre_ipropN = Binding.name "pre_iprop"
+  val resFN = Binding.name "resF"
+  val invN = Binding.name "inv"
+  val resN = Binding.name "res"
+  val ipropN = Binding.name "iprop"
+  val getter_prefix = "get_"
+  val constructor_prefix = "constr_"
+
+  (* Types *)
+  val invT = \<^typ>\<open>'a pre_inv\<close>
+  val heapT = \<^typ>\<open>heap_lang_heap\<close>
+  val cinvT = \<^typ>\<open>frac option\<close>
+  val aT = \<^typ>\<open>'a\<close>
+  val base_cameraT = HOLogic.mk_prodT (cinvT, HOLogic.mk_prodT (invT, heapT))
+  
+  fun mk_pred cmraT = typ_subst_atomic [(aT,cmraT)] \<^typ>\<open>'a upred_f\<close>
+  fun subst_aT fp cmraT = typ_subst_atomic [(aT,fp)] cmraT
+  fun add_cameraT cmraT cmrasT = HOLogic.mk_prodT (cmraT,cmrasT)
+  fun fixed_cmras preT = [
+    {camera = cinvT, name = "cinv", getter = NONE, constructor = NONE},
+    {camera = subst_aT preT invT, name = "inv", getter = NONE, constructor = NONE},
+    {camera = heapT, name = "heap", getter = NONE, constructor = NONE}
+   ]
+  val mk_cmraT = curry (Library.foldr (uncurry add_cameraT))
+
+  (* Setup to generate getters for single cameras from the camera product *)
+  fun mk_def trm lthy = let val prop_trm = HOLogic.mk_Trueprop trm
+    in Specification.definition NONE [] [] ((Binding.empty,[]), prop_trm) lthy |> snd end
+
+  fun mk_defs (cmras_data:cameras_data) lthy =
+    let fun mk_getter name cmraT = Free (getter_prefix ^ name, (the (#cmraPT cmras_data))-->cmraT)
+        fun mk_own name cmraT = Free (constructor_prefix ^ name, cmraT-->(the (#cmraPT cmras_data)))$
+          Free (Binding.name_of resN, cmraT)
+    in 
+      Library.foldl (fn (lthy, cmra_data:camera_data) => 
+        (mk_def (curry HOLogic.mk_eq (mk_getter (#name cmra_data) (#camera cmra_data)) 
+          (the (#getter cmra_data))) 
+       #> mk_def (curry HOLogic.mk_eq (mk_own (#name cmra_data) (#camera cmra_data)) 
+          (the (#constructor cmra_data))))
+       lthy)
+      (lthy, #cameras cmras_data)
+    end
+
+  val dummy_fst = Const (\<^const_name>\<open>fst\<close>, dummyT)
+  val dummy_snd = Const (\<^const_name>\<open>snd\<close>, dummyT)
+  val dummy_comp = Const (\<^const_name>\<open>comp\<close>, dummyT)
+  val dummy_I = Const (\<^const_name>\<open>id\<close>, dummyT)
+  val dummy_eps = Const (\<^const_name>\<open>\<epsilon>\<close>, dummyT)
+  val dummy_cmra_object = Free (Binding.name_of resN, dummyT)
+
+  fun mk_getter levels is_heap = 
+    let val base = if is_heap then dummy_I else dummy_fst
+      fun add_level 0 = base
+        | add_level n = dummy_comp$(add_level (n-1))$dummy_snd
+    in add_level levels end
+
+  fun mk_getters ({ number, cameras, cmraPT}: cameras_data) = let
+    fun mk_getters_levels _ _ [] = []
+      | mk_getters_levels levels n ((cmra: camera_data)::cameras) = 
+        {camera = #camera cmra, name = #name cmra,
+          getter= if n=levels then SOME (mk_getter n true) else SOME (mk_getter n false),
+          constructor = #constructor cmra
+        }::(mk_getters_levels levels (n+1) cameras)
+    in { number = number, cameras = mk_getters_levels (number-1) 0 cameras, cmraPT = cmraPT }
+    end
+
+  fun mk_own levels is_heap =
+    let val base = if is_heap then dummy_cmra_object 
+      else curry HOLogic.mk_prod dummy_cmra_object dummy_eps
+      fun add_level 0 = base
+        | add_level n = curry HOLogic.mk_prod dummy_eps (add_level (n-1))
+    in add_level levels end
+
+    fun mk_owns ({ number, cameras, cmraPT}: cameras_data) = let
+    fun mk_owns_levels _ _ [] = []
+      | mk_owns_levels levels n ((cmra: camera_data)::cameras) = 
+        {camera = #camera cmra, name = #name cmra,
+          getter = #getter cmra,
+          constructor = if n=levels then SOME (mk_own n true) else SOME (mk_own n false)
+        }::(mk_owns_levels levels (n+1) cameras)
+    in { number = number, cameras = mk_owns_levels (number-1) 0 cameras, cmraPT = cmraPT }
+    end
+
+  (* Setup functions *)
+  val mk_pre_iprop = Typedecl.typedecl_global {final=false} (pre_ipropN,[],NoSyn)
+
+  fun mk_axioms preT propT = 
+    [(iPropN,SOME (preT --> propT),NoSyn),(preN,SOME (propT --> preT) ,NoSyn)]
+  fun def_axioms ax_defs = (#2 o Specification.axiomatization ax_defs [] [] [])
+
+  fun def_resF cmraT = (#2 o Typedecl.abbrev_global (resFN,["'a", "'b"],NoSyn) cmraT)
+  fun def_inv preT = (#2 o Typedecl.abbrev_global (invN,[],NoSyn) (subst_aT preT invT))
+  fun def_res cmraT = (#2 o Typedecl.abbrev_global (resN,[],NoSyn) cmraT)
+  fun def_iprop cmraT = (#2 o Typedecl.abbrev_global (ipropN,[],NoSyn) (mk_pred cmraT))
+
+  (* Axiomatize that pre_iprop is of class ofe. This will mark the command with a red background. *)
+  fun pre_inst thy = Class.instance_arity_cmd ([Binding.name_of pre_ipropN], [], "ofe") thy
+    |> Proof.global_skip_proof false |> Proof_Context.theory_of
+  in
+
+  fun mk_iprop cmras thy = 
+    let val (preT,thy') = mk_pre_iprop thy 
+      val cmras_raw = map (fn (cmra,name)=>{camera=cmra, name=name, getter=NONE, constructor=NONE}) cmras
+      val cmra_data = {number = length cmras+3, cameras = cmras_raw@fixed_cmras preT, cmraPT = NONE}
+      val cmra_data = mk_getters cmra_data
+      val cmra_data = mk_owns cmra_data
+      val cmraT = subst_aT preT base_cameraT |> mk_cmraT (map fst cmras)
+      val propT = mk_pred cmraT 
+      val axs = mk_axioms preT propT
+      val cmra_data = {number = #number cmra_data, cameras = #cameras cmra_data, cmraPT = SOME cmraT}
+    in thy' |> Config.put_global quick_and_dirty true
+      |> def_axioms axs |> def_resF cmraT |> def_inv preT |> def_res cmraT |> def_iprop cmraT
+      |> pre_inst |> Named_Target.theory_map (mk_defs cmra_data)
+      |> Config.put_global quick_and_dirty false
+    end
+end;
+\<close>
+
+setup \<open>mk_iprop [(\<^typ>\<open>graphUR auth\<close>, "graph"), (\<^typ>\<open>markingUR auth\<close>, "markings")]\<close>
+
 lemma iprop_fp: "iProp (pre P) = P" sorry
 declare [[coercion iProp]]
 end
