HeapLang/HeapLang.thy
@@ -68,6 +68,8 @@ and val =
   | PairV val val
   | InjLV val
   | InjRV val
+
+declare [[coercion Val]]
   
 (* An observation associates a prophecy variable (identifier) to a pair of values. *)
 type_synonym observation = "proph_id * val * val"
