IrisCore/Namespace.thy
@@ -10,7 +10,12 @@ type_synonym namespace = "nat list"
 type_synonym name = "nat list"
 definition names :: "namespace \<Rightarrow> name set" where
   "names N = {n. \<exists>p. n=N@p}" \<comment> \<open> A namespace is used as the prefix for other names. \<close> 
-  
+
+definition nroot :: namespace where "nroot = []"
+definition add_name :: "namespace \<Rightarrow> name \<Rightarrow> namespace" where "add_name N n = N@n"
+definition string_to_name :: "string \<Rightarrow> name" where 
+  "string_to_name = (map nat_of_integer) \<circ> String.asciis_of_literal \<circ> String.implode"
+
 definition subnamespace :: "namespace \<Rightarrow> namespace \<Rightarrow> bool" where
   "subnamespace N1 N2 \<equiv> \<exists>p. N1=N2@p"
 lemma sub_names: "subnamespace N1 N2 \<longleftrightarrow> N1 \<in> names N2"
